src/tosyntax/FStarC.ToSyntax.ToSyntax.fsti
@@ -14,7 +14,6 @@
   limitations under the License.
 *)
 module FStarC.ToSyntax.ToSyntax
-#push-options "--MLish --MLish_effect FStarC.Effect"
 open FStarC.Effect
 
 open FStarC
@@ -28,34 +27,34 @@ open FStarC.Ident
 
 module S = FStarC.Syntax.Syntax
 
-type extension_tosyntax_decl_t = env -> FStarC.Dyn.dyn -> lids:list lident -> Range.t -> list sigelt'
-val register_extension_tosyntax (lang_name:string) (cb:extension_tosyntax_decl_t) : unit
+type extension_tosyntax_decl_t = env -> FStarC.Dyn.dyn -> lids:list lident -> Range.t -> ML (list sigelt')
+val register_extension_tosyntax (lang_name:string) (cb:extension_tosyntax_decl_t) : ML unit
+
+(* Return a list of wildcard patterns (implicit or explicit as needed)
+in order to expand the `..` in `| C .. ->`. *)
+val rest_pat_for_lid (env : env) (l : lid) : ML (list pattern)
 
 (* Only called from tactics *)
-val desugar_term:            env -> term -> S.term
+val desugar_term:            env -> term -> ML S.term
 
 val desugar_machine_integer: env -> repr:string
                            -> (FStarC.Const.signedness & FStarC.Const.width)
-                           -> Range.t -> Syntax.term
+                           -> Range.t -> ML Syntax.term
 
-val ast_modul_to_modul:          AST.modul -> withenv Syntax.modul
-val decls_to_sigelts:            list AST.decl -> withenv sigelts
-val partial_ast_modul_to_modul:  option S.modul -> AST.modul -> withenv Syntax.modul
+val parse_attr_with_list : bool -> S.term -> lident -> ML (option (list int & Range.t) & bool)
+
+val get_fail_attr1 : bool -> S.term       -> ML (option (list int & Range.t & bool))
+val get_fail_attr  : bool -> list S.term -> ML (option (list int & Range.t & bool))
+
+val ast_modul_to_modul:          AST.modul -> ML (withenv Syntax.modul)
+val decls_to_sigelts:            list AST.decl -> ML (withenv sigelts)
+val partial_ast_modul_to_modul:  option S.modul -> AST.modul -> ML (withenv Syntax.modul)
 
 val add_partial_modul_to_env: Syntax.modul
                     -> module_inclusion_info
                     -> erase_univs:(S.term -> S.term)
-                    -> withenv unit
+                    -> ML (withenv unit)
 val add_modul_to_env: Syntax.modul
                     -> module_inclusion_info
                     -> erase_univs:(S.term -> S.term)
-                    -> withenv unit
-
-val parse_attr_with_list : bool -> S.term -> lident -> option (list int & Range.t) & bool
-
-val get_fail_attr1 : bool -> S.term       -> option (list int & Range.t & bool)
-val get_fail_attr  : bool -> list S.term -> option (list int & Range.t & bool)
-
-(* Return a list of wildcard patterns (implicit or explicit as needed)
-in order to expand the `..` in `| C .. ->`. *)
-val rest_pat_for_lid (env : env) (l : lid) : list pattern
+                    -> ML (withenv unit)
